update the ds_abs1.rx automaton and finished the non-tau proofs

ds_abs1/ds_abs1_rxScript.sml
@@ -12,7 +12,8 @@ SPI_ABS1_RX_ENABLE (ds_abs1:ds_abs1_state) =
 (ds_abs1.ds_abs1_rx.state = abs1_rx_update) \/
 (ds_abs1.ds_abs1_rx.state = abs1_rx_fetch_data) \/
 (ds_abs1.ds_abs1_rx.state = abs1_rx_return) \/
-(ds_abs1.ds_abs1_rx.state = abs1_rx_ready_for_reset))`
+(ds_abs1.ds_abs1_rx.state = abs1_rx_check_1) \/
+(ds_abs1.ds_abs1_rx.state = abs1_rx_pre_reset))`
 
 (* DRIVER_ABS1_RX_ENABLE: ds_abs1_state -> bool *)
 val DRIVER_ABS1_RX_ENABLE_def = Define `
@@ -23,13 +24,22 @@ DRIVER_ABS1_RX_ENABLE (ds_abs1:ds_abs1_state) =
 (ds_abs1.ds_abs1_rx.state = abs1_rx_ready) \/
 (ds_abs1.ds_abs1_rx.state = abs1_rx_fetch_data) \/
 (ds_abs1.ds_abs1_rx.state = abs1_rx_return) \/
-(ds_abs1.ds_abs1_rx.state = abs1_rx_done))`
+(ds_abs1.ds_abs1_rx.state = abs1_rx_done) \/
+(ds_abs1.ds_abs1_rx.state = abs1_rx_check_1) \/
+(ds_abs1.ds_abs1_rx.state = abs1_rx_check_2))`
 
 (* COMB_ABS1_RX_ENABLE: ds_abs1_state -> bool *)
 val COMB_ABS1_RX_ENABLE_def = Define `
 COMB_ABS1_RX_ENABLE (ds_abs1:ds_abs1_state) =
 ((ds_abs1.ds_abs1_rx.state = abs1_rx_reset) \/
 (ds_abs1.ds_abs1_rx.state = abs1_rx_ready_for_reset))`
+
+(* ABS1_RX_LBL_ENABLE: ds_abs1_state -> bool *)
+val ABS1_RX_LBL_ENABLE_def = Define `
+ABS1_RX_LBL_ENABLE (ds_abs1:ds_abs1_state) =
+((ds_abs1.ds_abs1_rx.state = abs1_rx_receive) \/
+(ds_abs1.ds_abs1_rx.state = abs1_rx_done) \/
+(ds_abs1.ds_abs1_rx.state = abs1_rx_last))`
 
 (* tau_spi related functions *)
 (* spi_abs1_rx_idle_op: ds_abs1_state -> ds_abs1_state *)
@@ -58,9 +68,15 @@ spi_abs1_rx_return_op (ds_abs1:ds_abs1_state) =
 ds_abs1 with ds_abs1_rx := ds_abs1.ds_abs1_rx with
 state := abs1_rx_receive`
 
-(* spi_abs1_rx_ready_for_reset_op: ds_abs1_state -> ds_abs1_state *)
-val spi_abs1_rx_ready_for_reset_op_def = Define `
-spi_abs1_rx_ready_for_reset_op (ds_abs1:ds_abs1_state) =
+(* spi_abs1_rx_check_1_op: ds_abs1_state -> ds_abs1_state *)
+val spi_abs1_rx_check_1_op_def = Define `
+spi_abs1_rx_check_1_op (ds_abs1:ds_abs1_state) =
+ds_abs1 with ds_abs1_rx := ds_abs1.ds_abs1_rx with
+state := abs1_rx_check_2`
+
+(* spi_abs1_rx_pre_reset_op: ds_abs1_state -> ds_abs1_state *)
+val spi_abs1_rx_pre_reset_op_def = Define `
+spi_abs1_rx_pre_reset_op (ds_abs1:ds_abs1_state) =
 ds_abs1 with ds_abs1_rx := ds_abs1.ds_abs1_rx with
 state := abs1_rx_reset`
 
@@ -76,7 +92,11 @@ case ds_abs1.ds_abs1_rx.state of
   | abs1_rx_fetch_data => spi_abs1_rx_fetch_data_op ds_abs1
   | abs1_rx_return => spi_abs1_rx_return_op ds_abs1
   | abs1_rx_done => ds_abs1 with err := T
-  | abs1_rx_ready_for_reset => spi_abs1_rx_ready_for_reset_op ds_abs1
+  | abs1_rx_last => ds_abs1 with err := T
+  | abs1_rx_check_1 => spi_abs1_rx_check_1_op ds_abs1
+  | abs1_rx_check_2 => ds_abs1 with err := T
+  | abs1_rx_pre_reset => spi_abs1_rx_pre_reset_op ds_abs1
+  | abs1_rx_ready_for_reset => ds_abs1 with err := T
   | abs1_rx_reset => ds_abs1 with err := T`
 
 
@@ -141,6 +161,26 @@ ds_abs1 with ds_abs1_rx := ds_abs1.ds_abs1_rx with
    rx_data_buffer := ds_abs1.ds_abs1_rx.rx_data_buffer ++ [ds_abs1.spi_abs1.RX_SHIFT_REG];
    rx_left_length := ds_abs1.ds_abs1_rx.rx_left_length - 1 |>`
 
+(* driver_abs1_rx_check_1_op: ds_abs1_state -> ds_abs1_state *)
+val driver_abs1_rx_check_1_op_def = Define `
+driver_abs1_rx_check_1_op (ds_abs1: ds_abs1_state) =
+ds_abs1 with ds_abs1_rx := ds_abs1.ds_abs1_rx with 
+<| state := if ds_abs1.ds_abs1_rx.rx_left_length > 1 then abs1_rx_update
+   else abs1_rx_pre_reset;
+   rx_data_buffer := ds_abs1.ds_abs1_rx.rx_data_buffer ++ 
+                     [(w2w (THE ds_abs1.driver_abs1.dr_abs1_last_read_v):word8)];
+   rx_left_length := ds_abs1.ds_abs1_rx.rx_left_length - 1 |>`
+
+(* driver_abs1_rx_check_2_op: ds_abs1_state -> ds_abs1_state *)
+val driver_abs1_rx_check_2_op_def = Define `
+driver_abs1_rx_check_2_op (ds_abs1: ds_abs1_state) =
+ds_abs1 with ds_abs1_rx := ds_abs1.ds_abs1_rx with
+<| state := if ds_abs1.ds_abs1_rx.rx_left_length > 1 then abs1_rx_ready
+   else abs1_rx_reset;
+   rx_data_buffer := ds_abs1.ds_abs1_rx.rx_data_buffer ++
+                     [(w2w (THE ds_abs1.driver_abs1.dr_abs1_last_read_v):word8)];
+   rx_left_length := ds_abs1.ds_abs1_rx.rx_left_length - 1 |>`
+
 (* driver_abs1_rx_operations: ds_abs1_state -> ds_abs1_state *)
 val driver_abs1_rx_operations_def = Define `
 driver_abs1_rx_operations (ds_abs1:ds_abs1_state) =
@@ -153,6 +193,10 @@ case ds_abs1.ds_abs1_rx.state of
   | abs1_rx_fetch_data => driver_abs1_rx_fetch_data_op ds_abs1
   | abs1_rx_return => driver_abs1_rx_return_op ds_abs1
   | abs1_rx_done => driver_abs1_rx_done_op ds_abs1
+  | abs1_rx_last => ds_abs1 with err := T
+  | abs1_rx_check_1 => driver_abs1_rx_check_1_op ds_abs1
+  | abs1_rx_check_2 => driver_abs1_rx_check_2_op ds_abs1
+  | abs1_rx_pre_reset => ds_abs1 with err := T
   | abs1_rx_ready_for_reset => ds_abs1 with err := T
   | abs1_rx_reset => ds_abs1 with err := T`
 
@@ -193,5 +237,35 @@ ds_abs1 with
 <| ds_abs1_rx := ds_abs1.ds_abs1_rx with state := abs1_rx_update;
    spi_abs1 := ds_abs1.spi_abs1 with RX_SHIFT_REG := THE data |>
 else ds_abs1`
+
+(* abs1_rx_done_op: ds_abs1_state -> word8 option -> ds_abs1_state *)
+val abs1_rx_done_op_def = Define `
+abs1_rx_done_op (ds_abs1:ds_abs1_state) (data:word8 option) =
+if (data <> NONE) then
+ds_abs1 with 
+<| ds_abs1_rx := ds_abs1.ds_abs1_rx with state := abs1_rx_check_1;
+   spi_abs1 := ds_abs1.spi_abs1 with RX_SHIFT_REG := THE data;
+   driver_abs1 := ds_abs1.driver_abs1 with
+   <| dr_abs1_last_read_ad := (SOME SPI0_RX0); 
+   dr_abs1_last_read_v := (SOME (w2w ds_abs1.spi_abs1.RX_SHIFT_REG)) |> |>
+else ds_abs1`
+
+(* abs1_rx_last_op: ds_abs1_state -> word8 option -> ds_abs1_state *)
+val abs1_rx_last_op_def = Define `
+abs1_rx_last_op (ds_abs1:ds_abs1_state) (data:word8 option) =
+if (data <> NONE) then
+ds_abs1 with 
+<| ds_abs1_rx := ds_abs1.ds_abs1_rx with state := abs1_rx_pre_reset;
+   spi_abs1 := ds_abs1.spi_abs1 with RX_SHIFT_REG := THE data |>
+else ds_abs1`
+
+
+(* abs1_rx_receive_data_op: ds_abs1_state -> word8 option -> ds_abs1_state *)
+val abs1_rx_receive_data_op_def = Define `
+abs1_rx_receive_data_op (ds_abs1:ds_abs1_state) (data:word8 option) =
+if ds_abs1.ds_abs1_rx.state = abs1_rx_receive then (abs1_rx_receive_op ds_abs1 data)
+else if ds_abs1.ds_abs1_rx.state = abs1_rx_done then (abs1_rx_done_op ds_abs1 data)
+else if ds_abs1.ds_abs1_rx.state = abs1_rx_last then (abs1_rx_last_op ds_abs1 data)
+else ds_abs1 with err := T`
 
 val _ = export_theory();
